IIO seems defined ok, but the lift from IO to IIO is admitted

IIO.Effect.fst
@@ -26,13 +26,13 @@ let rec iio_interpretation #a
 
 
 // REFINED COMPUTATION MONAD (repr)
-let irepr (a:Type) (wp:io_wpty a) =
+let iio_irepr (a:Type) (wp:io_wpty a) =
   h:events_trace -> post:io_post a ->
     Pure (iio a)
       (requires (wp h post))
       (ensures (fun (t:iio a) -> iio_interpretation t h post))
 
-let ireturn (a : Type) (x : a) : irepr a (io_return_wp a x) =
+let iio_ireturn (a : Type) (x : a) : iio_irepr a (io_return_wp a x) =
   fun _ _ -> iio_return a x
 
 let w = io_wpty
@@ -41,8 +41,8 @@ unfold
 val w_ord (#a : Type) : w a -> w a -> Type0
 let w_ord wp1 wp2 = forall h p. wp1 h p ==> wp2 h p
 
-let ibind (a b : Type) (wp_v : w a) (wp_f: a -> w b) (v : irepr a wp_v)
-  (f : (x:a -> irepr b (wp_f x))) : irepr b (io_bind_wp _ _ wp_v wp_f) =
+let iio_ibind (a b : Type) (wp_v : w a) (wp_f: a -> w b) (v : iio_irepr a wp_v)
+  (f : (x:a -> iio_irepr b (wp_f x))) : iio_irepr b (io_bind_wp _ _ wp_v wp_f) =
   fun h p -> 
     let t = (iio_bind a b 
         (v h (compute_post a b h wp_f p))
@@ -53,16 +53,16 @@ let ibind (a b : Type) (wp_v : w a) (wp_f: a -> w b) (v : irepr a wp_v)
     t
 
 unfold
-let isubcomp (a:Type) (wp1 wp2: w a) (f : irepr a wp1) :
-  Pure (irepr a wp2) (requires w_ord wp2 wp1) (ensures fun _ -> True) = f
+let isubcomp (a:Type) (wp1 wp2: w a) (f : iio_irepr a wp1) :
+  Pure (iio_irepr a wp2) (requires w_ord wp2 wp1) (ensures fun _ -> True) = f
 
 unfold
 let wp_if_then_else (#a:Type) (wp1 wp2:w a) (b:bool) : w a =
   fun h p -> (b ==> wp1 h p) /\ ((~b) ==> wp2 h p)
 
 unfold
-let i_if_then_else (a : Type) (wp1 wp2 : w a) (f : irepr a wp1) (g : irepr a wp2) (b : bool) : Type =
-  irepr a (wp_if_then_else wp1 wp2 b)
+let i_if_then_else (a : Type) (wp1 wp2 : w a) (f : iio_irepr a wp1) (g : iio_irepr a wp2) (b : bool) : Type =
+  iio_irepr a (wp_if_then_else wp1 wp2 b)
 
 total
 reifiable
@@ -70,26 +70,35 @@ reflectable
 layered_effect {
   IIOwp : a:Type -> wp : io_wpty a -> Effect
   with
-       repr       = irepr
-     ; return     = ireturn
-     ; bind       = ibind
+       repr       = iio_irepr
+     ; return     = iio_ireturn
+     ; bind       = iio_ibind
 
      ; subcomp      = isubcomp
      ; if_then_else = i_if_then_else
 }
 
 let lift_pure_iiowp (a:Type) (wp:pure_wp a) (f:(eqtype_as_type unit -> PURE a wp)) :
-  Pure (irepr a (fun s0 p -> wp (fun r -> p (Inl r) []))) (requires True)
+  Pure (iio_irepr a (fun s0 p -> wp (fun r -> p (Inl r) []))) (requires True)
                     (ensures (fun _ -> True))
   = fun s0 p -> let r = elim_pure f (fun r -> p (Inl r) []) in iio_return _ r
 
 sub_effect PURE ~> IOwp = lift_pure_iowp
 
-let lift_iowp_iiowp (a:Type) (wp:io_wpty a) (f:IO.Effect.irepr a wp) :
-  Pure (irepr a (fun s0 p -> wp s0 (fun r le -> p r le))) 
+// let rec cast_io_iio #a (x:io a) : iio a =
+//   match x with
+//   | Return z -> Return z
+//   | Throw z -> Throw z
+//   | Cont (Call cmd args fnc) ->
+//          Cont (Call cmd args (fun res ->
+//            FStar.WellFounded.axiom1 fnc res;
+//            cast_io_iio (fnc res)))
+
+let lift_iowp_iiowp (a:Type) (wp:io_wpty a) (f:io_irepr a wp) :
+  Pure (iio_irepr a (fun s0 p -> wp s0 (fun r le -> p r le))) 
     (requires True)
     (ensures (fun _ -> True))
-  // TODO: lift from IO.irepr to IIO.irepr
+  // TODO: lift from IO.irepr to IIO.iio_irepr
   = fun s0 p -> admit (); f s0 p
 
 sub_effect IOwp ~> IIOwp = lift_iowp_iiowp
@@ -101,25 +110,66 @@ effect IIO
   IIOwp a (fun (h:events_trace) (p:io_post a) ->
     pre h /\ (forall res le. post h res le ==>  p res le))
 
-let openfile = static_cmd Openfile
-let read = static_cmd Read
-let close = static_cmd Close
+let get_trace () : IIO events_trace (fun h -> True) 
+  (fun h r le -> r == (Inl h) /\ le == []) =
+  IIOwp?.reflect (fun _ _ -> sys_perform (Call GetTrace () (fun h -> h)))
 
-let testStat2 () : 
-  IIO unit (fun h -> True) (fun h _ le -> enforced_locally default_check h le) =
-  let fd = openfile "../Makefile" in
-  let msg = read fd in
-  close fd;
-  ()
+let throw (err:exn) : IIOwp events_trace (fun _ p -> p (Inr err) []) =
+  IIOwp?.reflect(fun _ _ -> iio_throw _ err)
 
-let get () : IIO events_trace (fun h -> True) 
-  (fun h r le -> r == (Inl h)) by (
-  let h = forall_intro () in
-  let p = forall_intro () in
-  norm [delta_only[`%iio_interpretation]];
-  let _ = forall_intro () in
-  let g = implies_intro () in
-  let l1, l2 = Tactics.destruct_and g in
-  dump "h") =
-  IIOwp?.reflect (fun _ _ -> iio_all GetTrace ())
+let pi_static_cmd
+  (cmd : io_cmds)
+  (pi : monitorable_prop)
+  (arg : args cmd) :
+  IIO (res cmd)
+    (requires (fun h ->
+      default_check h (| cmd, arg |) &&
+      pi h (| cmd, arg |)))
+    (ensures (fun h r le ->
+      (match r with
+      | Inr GIO_pi_failed -> False
+      | Inr GIO_default_check_failed -> False
+      | _ -> le == [convert_call_to_event cmd arg r])
+      /\ enforced_locally default_check h le
+      /\ enforced_locally pi h le)) =
+  static_cmd cmd arg
 
+let mixed_cmd
+  (cmd : io_cmds)
+  (pi : monitorable_prop)
+  (arg : args cmd) :
+  IIO (res cmd)
+    (requires (fun s0 -> default_check s0 (| cmd, arg |)))
+    (ensures (fun h r le ->
+      (match r with
+      | Inr GIO_default_check_failed -> False
+      | Inr GIO_pi_failed -> le == []
+      | _ -> le == [convert_call_to_event cmd arg r])
+      /\ enforced_locally default_check h le
+      /\ enforced_locally pi h le
+      )) =
+  let s0 = get_trace () in
+  let action = (| cmd, arg |) in
+  match pi s0 action with
+  | true -> pi_static_cmd cmd pi arg
+  | false -> throw GIO_pi_failed
+
+let dynamic_cmd
+  (cmd : io_cmds)
+  (pi : monitorable_prop)
+  (arg : args cmd) :
+  IIO (res cmd) 
+    (requires (fun s0 -> True))
+    (ensures (fun h r le ->
+      (match r with
+      | Inr GIO_default_check_failed
+      | Inr GIO_pi_failed -> le == []
+      | _ -> le == [convert_call_to_event cmd arg r])
+      /\ enforced_locally default_check h le
+      /\ enforced_locally pi h le
+  )) =
+  let s0 = get_trace () in
+  let action = (| cmd, arg |) in
+  match default_check s0 action with
+  | true -> mixed_cmd cmd pi arg
+  | false -> throw GIO_default_check_failed
