IO.Effect.fst
@@ -39,6 +39,11 @@ unfold let convert_call_to_event (cmd:io_cmds) (args:args cmd) (res:resm cmd) =
   | Read -> ERead args res
   | Close -> EClose args res
 
+// It is weird that this interpretation knows about
+// contract failure. Somebody will be able to throw this errors
+// manually so, I don't think this is the best place to do them.
+// Probably it will be better to refine the output of the `io_all`
+// than to modify the interpretation here.
 let rec io_interpretation #a
   (m : io a) 
   (p : io_post a) : Type0 = 
@@ -46,20 +51,20 @@ let rec io_interpretation #a
   | Return x -> p (Inl x) []
   | Throw err -> p (Inr err) []
   | Cont (Call cmd args fnc) -> (
-    forall res. (
+    forall res. (Inr? res ==>  ~(Inr?.v res == GIO_pi_failed \/ Inr?.v res == GIO_default_check_failed)) ==> (
       FStar.WellFounded.axiom1 fnc res;
       let event : io_event = convert_call_to_event cmd args res in
       io_interpretation (fnc res) (gen_post p event)))
 
 
 // REFINED COMPUTATION MONAD (repr)
-let irepr (a:Type) (wp:io_wpty a) =
+let io_irepr (a:Type) (wp:io_wpty a) =
   h:events_trace -> post:io_post a ->
     Pure (io a)
       (requires (wp h post))
       (ensures (fun (t:io a) -> io_interpretation t post))
 
-let ireturn (a : Type) (x : a) : irepr a (io_return_wp a x) =
+let io_ireturn (a : Type) (x : a) : io_irepr a (io_return_wp a x) =
   fun _ _ -> io_return a x
 
 let w = io_wpty
@@ -72,8 +77,8 @@ unfold
 let apply_changes (old_state local_trace:events_trace) = (List.rev local_trace) @ old_state
 
 
-let ibind (a b : Type) (wp_v : w a) (wp_f: a -> w b) (v : irepr a wp_v)
-  (f : (x:a -> irepr b (wp_f x))) : irepr b (io_bind_wp _ _ wp_v wp_f) =
+let io_ibind (a b : Type) (wp_v : w a) (wp_f: a -> w b) (v : io_irepr a wp_v)
+  (f : (x:a -> io_irepr b (wp_f x))) : io_irepr b (io_bind_wp _ _ wp_v wp_f) =
   fun h p -> 
     let t = (io_bind a b 
         (v h (compute_post a b h wp_f p))
@@ -84,16 +89,16 @@ let ibind (a b : Type) (wp_v : w a) (wp_f: a -> w b) (v : irepr a wp_v)
     t
 
 unfold
-let isubcomp (a:Type) (wp1 wp2: w a) (f : irepr a wp1) :
-  Pure (irepr a wp2) (requires w_ord wp2 wp1) (ensures fun _ -> True) = f
+let isubcomp (a:Type) (wp1 wp2: w a) (f : io_irepr a wp1) :
+  Pure (io_irepr a wp2) (requires w_ord wp2 wp1) (ensures fun _ -> True) = f
 
 unfold
 let wp_if_then_else (#a:Type) (wp1 wp2:w a) (b:bool) : w a =
   fun h p -> (b ==> wp1 h p) /\ ((~b) ==> wp2 h p)
 
 unfold
-let i_if_then_else (a : Type) (wp1 wp2 : w a) (f : irepr a wp1) (g : irepr a wp2) (b : bool) : Type =
-  irepr a (wp_if_then_else wp1 wp2 b)
+let i_if_then_else (a : Type) (wp1 wp2 : w a) (f : io_irepr a wp1) (g : io_irepr a wp2) (b : bool) : Type =
+  io_irepr a (wp_if_then_else wp1 wp2 b)
 
 total
 reifiable
@@ -101,16 +106,16 @@ reflectable
 layered_effect {
   IOwp : a:Type -> wp : io_wpty a -> Effect
   with
-       repr       = irepr
-     ; return     = ireturn
-     ; bind       = ibind
+       repr       = io_irepr
+     ; return     = io_ireturn
+     ; bind       = io_ibind
 
      ; subcomp      = isubcomp
      ; if_then_else = i_if_then_else
 }
 
 let lift_pure_iowp (a:Type) (wp:pure_wp a) (f:(eqtype_as_type unit -> PURE a wp)) :
-  Pure (irepr a (fun s0 p -> wp (fun r -> p (Inl r) []))) (requires True)
+  Pure (io_irepr a (fun s0 p -> wp (fun r -> p (Inl r) []))) (requires True)
                     (ensures (fun _ -> True))
   = fun s0 p -> let r = elim_pure f (fun r -> p (Inl r) []) in io_return _ r
 
@@ -143,25 +148,17 @@ let default_check (state:events_trace) (action:action_type) =
   | (| Read, fd |) -> is_open fd state
   | (| Close, fd |) -> is_open fd state
 
-
 let static_cmd
   (cmd : io_cmds)
   (argz : io_args cmd) :
   IO (res cmd)
     (requires (fun h -> default_check h (| cmd, argz |)))
     (ensures (fun h r local_trace ->
+      (match r with
+      | Inr GIO_pi_failed -> False
+      | Inr GIO_default_check_failed -> False
+      | _ -> True) /\
       local_trace == [convert_call_to_event cmd argz r]
       /\ enforced_locally default_check h local_trace
-  )) =
+  )) by (compute ()) =
   IOwp?.reflect(fun _ _ -> io_all cmd argz)
-
-let openfile = static_cmd Openfile
-let read = static_cmd Read
-let close = static_cmd Close
-
-let testStat2 () : 
-  IO unit (fun h -> True) (fun h _ le -> enforced_locally default_check h le) =
-  let fd = openfile "../Makefile" in
-  let msg = read fd in
-  close fd;
-  ()
