Common.fst
@@ -2,6 +2,9 @@ module Common
 
 open FStar.Exn
 
+exception GIO_default_check_failed
+exception GIO_pi_failed
+
 type maybe a = either a exn
 
 type file_descr = int
